Prove b_refillBuffer_with_input_spec

basis/TextIOProofScript.sml
@@ -574,7 +574,7 @@ val REF_NUM_def = Define `
     SEP_EXISTS v. REF loc v * & (NUM n v)`;
 
 val instream_buffered_inv_def = Define `
-  instream_buffered_inv r w bcontent wrarea bactive =
+  instream_buffered_inv r w bcontent bactive =
       (1028 <= LENGTH bcontent  /\
        LENGTH bcontent < 256**2 /\
       4 <= w /\
@@ -582,15 +582,14 @@ val instream_buffered_inv_def = Define `
       r <= LENGTH bcontent /\
       w <= LENGTH bcontent /\
       r <= w /\
-      wrarea = DROP 4 bcontent /\
       bactive = TAKE (w-r) (DROP r bcontent))`;
 
 val INSTREAM_BUFFERED_def = Define `
   INSTREAM_BUFFERED bactive is =
-    SEP_EXISTS rr r wr w buff bcontent wrarea fd fdv.
+    SEP_EXISTS rr r wr w buff bcontent fd fdv.
       & (is = (Conv (SOME (TypeStamp "InstreamBuffered" 11)) [fdv; rr; wr; buff]) /\
         INSTREAM fd fdv /\
-        instream_buffered_inv r w bcontent wrarea bactive) *
+        instream_buffered_inv r w bcontent bactive) *
       REF_NUM rr r *
       REF_NUM wr w *
       W8ARRAY buff bcontent`;
@@ -1838,7 +1837,6 @@ Theorem b_openInSetBufferSize_spec
     \\map_every qexists_tac [`4`, `4`]
     \\fs[instream_buffered_inv_def, MAX_DEF] \\ xsimpl);
 
-
 Theorem b_openIn_spec
   `∀s sv fs bactive.
      FILENAME s sv ∧
@@ -1856,6 +1854,9 @@ Theorem b_openIn_spec
   (xcf_with_def "TextIO.b_openIn" TextIO_b_openIn_v_def
   \\xapp \\ fs[INT_NUM_EXISTS]);
 
+val take_fromI_def = Define `
+  take_fromI n content pos = TAKE n (DROP pos (MAP (n2w o ORD) content))`;
+
 Theorem b_refillBuffer_with_input_spec
   `!fd fdv fs content pos.
     INSTREAM fd fdv  ∧
@@ -1866,10 +1867,10 @@ Theorem b_refillBuffer_with_input_spec
     (STDIO fs * INSTREAM_BUFFERED bactive is )
     (POSTv wv. SEP_EXISTS wrAreaSize.
                   &(NUM (MIN wrAreaSize (LENGTH content - pos)) wv) *
-                  INSTREAM_BUFFERED (TAKE (MIN wrAreaSize (LENGTH content - pos))
-                                      (DROP pos (MAP (n2w o ORD) content))) is *
+                  INSTREAM_BUFFERED (take_fromI wrAreaSize content pos) is *
         STDIO (fsupdate fs fd 0 (MIN (wrAreaSize + pos) (MAX pos (LENGTH content))) content))`
   (xcf_with_def "TextIO.b_refillBuffer_with_input" TextIO_b_refillBuffer_with_input_v_def
+  \\rw[take_fromI_def]
   \\qpat_abbrev_tac`fcontent = (MAP (n2w o ORD) content)`
   \\fs[INSTREAM_BUFFERED_def, REF_NUM_def]
   \\xpull
@@ -1886,39 +1887,35 @@ Theorem b_refillBuffer_with_input_spec
   \\xapp \\ xsimpl
   \\qexists_tac `&((MIN (LENGTH bcontent - 4) (STRLEN content − pos)) + 4)`  \\fs[NUM_def, MIN_DEF]
   \\rpt strip_tac
-  \\map_every qexists_tac [`LENGTH bcontent-4`,`(MIN (LENGTH bcontent-4) (STRLEN content − pos))`,`fd`]
+  \\map_every qexists_tac [`LENGTH bcontent - 4`,`(MIN (LENGTH bcontent - 4) (STRLEN content − pos)) + 4`,`fd`]
   \\simp[MAX_DEF,MIN_DEF] \\ fs[INT_SUB_CALCULATE, INT_ADD_CALCULATE] \\ xsimpl
   \\qpat_abbrev_tac`take_fcontent = (TAKE (LENGTH bcontent - 4) (DROP pos fcontent))`
   \\`LENGTH take_fcontent <= LENGTH bcontent` by
       fs[Abbr`take_fcontent`,Abbr`fcontent`,LENGTH_TAKE_EQ_MIN,LENGTH_TAKE,MIN_DEF]
-  `1028 ≤ LENGTH (insert_atI take_fcontent 4 bcontent)` by fs[insert_atI_def] \\ simp[]
-   `LENGTH (insert_atI take_fcontent 4 bcontent) < 65536` by fs[LENGTH_insert_atI] \\ simp[]
-  \\fs[LENGTH_insert_atI]
+  \\`LENGTH take_fcontent <= LENGTH bcontent - 4` by
+      fs[Abbr`take_fcontent`,Abbr`fcontent`,LENGTH_TAKE_EQ_MIN,LENGTH_TAKE,MIN_DEF]
+  \\`LENGTH take_fcontent + 4 <= LENGTH bcontent` by fs[INT_LE_SUB_LADD]
+  \\ fs[LENGTH_insert_atI]
   \\CASE_TAC
+  >-(simp[Abbr`take_fcontent`,insert_atI_def,Abbr`fcontent`,TAKE_APPEND, DROP_APPEND]
+    \\simp[DROP_SEG, SEG]
+    \\simp[TAKE_TAKE_T, LENGTH_TAKE])
   >-(rw[Abbr`take_fcontent`,insert_atI_def,TAKE_APPEND]
-    \\`LENGTH (TAKE (LENGTH bcontent) (DROP pos fcontent)) = LENGTH bcontent`
-            by fs[Abbr`fcontent`,LENGTH_TAKE]
-    \\fs[Abbr`fcontent`,TAKE_0,TAKE_TAKE])
-  >-(rw[Abbr`take_fcontent`,insert_atI_def,TAKE_APPEND]
-    \\`LENGTH (TAKE (LENGTH bcontent) (DROP pos fcontent)) =
-          MIN (LENGTH bcontent) (LENGTH fcontent - pos)`
+    \\`LENGTH (TAKE (LENGTH bcontent-4) (DROP pos fcontent)) =
+          MIN (LENGTH bcontent-4) (LENGTH fcontent - pos)`
             by fs[Abbr`fcontent`,LENGTH_TAKE_EQ_MIN, LENGTH_DROP]
-    \\fs[MIN_DEF] \\ CASE_TAC
-    >-(fs[Abbr`fcontent`,take_drop_append])
-    >-(fs[Abbr`fcontent`,take_drop_append, TAKE_TAKE_MIN]
-      >-(fs[MIN_DEF] \\ CASE_TAC
-        >-(`STRLEN content - pos = LENGTH bcontent` by fs[]
-\\fs[])))));
-
-SUBGOAL_THEN ``LENGTH (insert_atI (take_fcontent:word8 list) 4 (bcontent:word8 list)) < 65536`` assume_tac
-fs[insert_atI_def]
-Cases_on `LENGTH take_fcontent + 4` >- fs[]
->-(Cases_on `LENGTH bcontent` >- fs[]
-  \\fs[GSYM SUC_ADD_SYM]
-  \\fs[SUC_ONE_ADD]
-  \\fs[SUB_EQUAL_0]
-  `n' - n + n = 0` by intLib.ARITH_TAC
-  `SUC n + (SUC n' − SUC n) =  SUC n + SUC n' − SUC n` by fs[SUB_LEFT_ADD])
+    \\simp[DROP_APPEND]
+    \\fs[MIN_DEF] \\ simp[DROP_SEG, SEG]
+    >-(CASE_TAC
+      >-(fs[Abbr`fcontent`,take_drop_append])
+      >-(fs[Abbr`fcontent`,take_drop_append, TAKE_TAKE_MIN]
+        \\fs[MIN_DEF] \\ simp[DROP_APPEND, DROP_SEG, SEG, TAKE_APPEND,
+                              TAKE_TAKE_T,TAKE_LENGTH_TOO_LONG]))
+    >-(CASE_TAC
+      >-(fs[Abbr`fcontent`,take_drop_append])
+      >-(fs[Abbr`fcontent`,take_drop_append, TAKE_TAKE_MIN]
+        \\fs[MIN_DEF] \\ simp[DROP_APPEND, DROP_SEG, SEG, TAKE_APPEND,
+                              TAKE_TAKE_T,TAKE_LENGTH_TOO_LONG]))));
 
 Theorem b_refillBuffer_with_read_spec
  `!fd fdv fs content pos.
@@ -1932,7 +1929,7 @@ Theorem b_refillBuffer_with_read_spec
                    buff = (0w::n2w (nr DIV 256)::n2w nr::h4'::rest)) *
                  INSTREAM_BUFFERED_FD (TAKE nr (DROP pos (MAP (n2w o ORD) content))) fd is *
        SEP_EXISTS k. IOFS_WO_iobuff (fsupdate fs fd k (nr+pos) content))`
-  (xcf_with_def "TextIO.b_refillBuffer" TextIO_b_refillBuffer_with_read_v_def
+  (xcf_with_def "TextIO.b_refillBuffer_with_read" TextIO_b_refillBuffer_with_read_v_def
   \\reverse(Cases_on`pos ≤ LENGTH content`)
     >-(imp_res_tac get_file_content_eof \\ rfs[]
       \\fs[MAX_DEF, MIN_DEF, IOFS_WO_iobuff_def,
